Fix more canonicalization proofs

Optimizations/Canonicalizations/ShiftPhase.thy
@@ -5,6 +5,203 @@ theory ShiftPhase
     Common
 begin
 
+subsection \<open>Integer\<close>
+
+text \<open>
+\begin{lstlisting}[language=java]
+
+class Long {
+    public static int numberOfLeadingZeros(long i) {
+        int x = (int)(i >>> 32);
+        return x == 0 ? 32 + Integer.numberOfLeadingZeros((int)i)
+                : Integer.numberOfLeadingZeros(x);
+    }
+}
+
+class Integer {
+    public static int numberOfLeadingZeros(int i) {
+        // HD, Count leading 0's
+        if (i <= 0)
+            return i == 0 ? 32 : 0;
+        int n = 31;
+        if (i >= 1 << 16) { n -= 16; i >>>= 16; }
+        if (i >= 1 <<  8) { n -=  8; i >>>=  8; }
+        if (i >= 1 <<  4) { n -=  4; i >>>=  4; }
+        if (i >= 1 <<  2) { n -=  2; i >>>=  2; }
+        return n - (i >>> 1);
+    }
+}
+\end{lstlisting}
+\<close>
+
+(*fun numberOfLeadingZeros :: "32 word \<Rightarrow> nat" where
+  "numberOfLeadingZeros i = 
+    (if i = 0 then 32 else 0)
+  "
+*)
+
+subsection \<open>CodeUtil\<close>
+
+text \<open>
+The @{text jdk.vm.ci.code.CodeUtil} class is used by the GraalVM compiler to perform
+non-standard operations on integers.
+\<close>
+
+paragraph \<open>CodeUtil.isPowerOf2\<close>
+text \<open>
+The isPowerOf2 determines if a long is a power of 2 through bit manipulation.
+Our encoding is based on it's definition.
+
+\begin{lstlisting}[language=java]
+public static boolean isPowerOf2(long val) {
+    return val > 0 && (val & val - 1) == 0;
+}
+\end{lstlisting}
+
+The isPowerOf2 operation is performed on longs,
+so we should be safe here to define our function in terms of a 64-bit word.
+\<close>
+
+fun CodeUtil_isPowerOf2 :: "64 word \<Rightarrow> bool" where
+  "CodeUtil_isPowerOf2 v = (0 <s v \<and> (and v (v - 1)) = 0)"
+
+lemma positive_powers:
+  "CodeUtil_isPowerOf2 v \<Longrightarrow> (0 <s v)"
+  by simp
+
+lemma some_bit_set:
+  fixes v :: "64 word"
+  assumes "v \<noteq> 0"
+  shows "\<exists>n. bit v n"
+  using assms
+  by (metis bit_and_iff bit_eqI word_log_esimps(7))
+
+lemma positive_bit_set_between:
+  fixes v :: "64 word"
+  assumes "0 <s v"
+  shows "\<exists>n. 0 \<le> n \<and> n < 64 \<and> bit v n"
+  using assms
+  by (metis ValueThms.size64 bit_imp_le_length less_eq_nat.simps(1) signed.dual_order.strict_implies_not_eq some_bit_set wsst_TYs(3))
+
+lemma has_set_bit:
+  assumes "CodeUtil_isPowerOf2 v"
+  shows "\<exists>n. 0 \<le> n \<and> n < 64 \<and> bit v n"
+  using assms unfolding CodeUtil_isPowerOf2.simps
+  using positive_bit_set_between by blast
+
+lemma all_other_unset:
+  assumes "CodeUtil_isPowerOf2 v"
+  shows "\<exists>n. 0 \<le> n \<and> n < 64 \<and> bit v n \<and> (\<forall>n'. n' \<noteq> n \<longrightarrow> \<not>(bit v n'))"
+proof -
+  obtain n where n: "0 \<le> n \<and> n < 64 \<and> bit v n"
+    using assms has_set_bit by presburger
+  have "\<forall>n'. n' \<noteq> n \<longrightarrow> \<not>(bit v n')"
+    using assms unfolding CodeUtil_isPowerOf2.simps sorry
+  then show ?thesis
+    using n by blast
+qed
+
+lemma distinct_bit:
+  assumes "CodeUtil_isPowerOf2 v"
+  assumes "bit v n"
+  assumes "bit v n'"
+  shows "n = n'"
+  using assms all_other_unset
+  by metis
+
+paragraph \<open>CodeUtil.log2\<close>
+text \<open>
+
+\begin{lstlisting}[language=java]
+public static int log2(long val) {
+    assert val > 0;
+    return (Long.SIZE - 1) - Long.numberOfLeadingZeros(val);
+}
+\end{lstlisting}
+\<close>
+
+fun CodeUtil_log2 :: "64 word \<Rightarrow> nat" where
+  "CodeUtil_log2 v = (64 - 1 - (numberOfLeadingZeros v))"
+
+lemma log2_highest_one_bit:
+  fixes v :: "64 word"
+  assumes "v > 0"
+  shows "CodeUtil_log2 v = nat (highestOneBit v)"
+proof -
+  have "highestOneBit v < 64"
+    using highestOneBit_top by auto
+  then show ?thesis
+  unfolding CodeUtil_log2.simps numberOfLeadingZeros_def
+  unfolding ValueThms.size64 by auto
+qed
+
+lemma log2_has_bit_set:
+  assumes "CodeUtil_log2 x = i"
+  assumes "x > 0"
+  shows "0 \<le> i \<and> i < 64 \<and> bit x i"
+  apply (rule conjI) defer apply (rule conjI) defer defer
+  using assms unfolding CodeUtil_log2.simps 
+  apply blast
+  using assms(1) apply fastforce
+  using assms log2_highest_one_bit highestOneBitElim
+  by (metis MaxOrNeg_def highestOneBitNeg highestOneBit_def less_le nat_int)
+
+
+paragraph \<open>Combine isPowerOf2 and log2\<close>
+
+lemma log2_powerOf2:
+  assumes "CodeUtil_isPowerOf2 x"
+  assumes "CodeUtil_log2 x = i"
+  shows "0 \<le> i \<and> i < 64 \<and> bit x i \<and> (\<forall>n'. n' \<noteq> i \<longrightarrow> \<not>(bit x n'))"
+  using assms distinct_bit
+  by (metis log2_has_bit_set positive_powers signed.dual_order.strict_implies_not_eq word_gt_0)
+
+lemma is_push_bit:
+  assumes "0 \<le> i \<and> i < 64 \<and> bit x i \<and> (\<forall>n'. n' \<noteq> i \<longrightarrow> \<not>(bit x n'))"
+  shows "x = push_bit i 1"
+  using assms unfolding bit_iff_odd push_bit_eq_mult apply auto sorry
+
+lemma log2_base:
+  assumes "CodeUtil_isPowerOf2 x"
+  assumes "CodeUtil_log2 x = i"
+  shows "x = 2^i"
+  using assms log2_powerOf2 push_bit_of_1 is_push_bit
+  by fastforce
+
+lemma shift_opt:
+  assumes "CodeUtil_isPowerOf2 x"
+  assumes "CodeUtil_log2 x = i"
+  shows "a * x = a << i"
+  using assms
+  by (metis log2_base shiftl_power)
+
+(*
+lemma
+  assumes "c > 0"
+  assumes "CodeUtil_isPowerOf2 c"
+  assumes "val[a * IntVal b c] \<noteq> UndefVal"
+  shows "val[a * IntVal b c] = val[a << IntVal b (word_of_nat (CodeUtil_log2 c))]"
+proof -
+  obtain av where "a = IntVal b av"
+    by (smt (z3) assms(3) intval_bits.simps intval_mul.elims new_int_bin.simps)
+  have "intval_mul a (IntVal b c) = IntVal b (take_bit b (av * c))"
+    by (simp add: \<open>a = IntVal b av\<close>)
+  have "intval_left_shift a (IntVal b (word_of_nat (CodeUtil_log2 c))) = IntVal b (take_bit b ((av << shift_amount b (word_of_nat (CodeUtil_log2 c)))))"
+    using \<open>a = IntVal b av\<close> eval_thms(90) new_int.simps by presburger
+  
+  then show ?thesis
+  proof (cases "b = 64")
+    case True
+    then show ?thesis sorry
+  next
+    case False
+    have "shift_amount b (word_of_nat (CodeUtil_log2 c)) = (CodeUtil_log2 c) mod 32"
+      using False unfolding shift_amount.simps apply (simp del: CodeUtil_log2.simps) using shift_amount_32 log2_has_bit_set sorry
+    then show ?thesis sorry
+  qed
+*)
+
+                                        
 phase ShiftNode
   terminating size
 begin
